specs/Spec.Lib.IntTypes.fst
@@ -1,0 +1,218 @@
+module Spec.Lib.IntTypes
+
+open FStar.Seq
+open FStar.Endianness
+
+(* Declared in .fsti : intsize, bits *)
+
+let uint_t (t:inttype) : Type0 = 
+  match t with
+  | U8 -> UInt8.t
+  | U16 -> UInt16.t
+  | U32 -> UInt32.t
+  | U64 -> UInt64.t
+  | U128 -> UInt128.t
+    
+noeq type uint_ =
+ | UInt: t:inttype -> v:uint_t t -> uint_
+
+let uint = uint_
+let ty u = u.t
+
+let uint_v (u:uint) = 
+  match u with
+  | UInt U8 x -> UInt8.v x
+  | UInt U16 x -> UInt16.v x
+  | UInt U32 x -> UInt32.v x
+  | UInt U64 x -> UInt64.v x
+  | UInt U128 x -> UInt128.v x
+
+
+(* Declared in .fsti: uint8, uint16, uint32, uint64, uint128 *)
+
+let u8 (x:UInt8.t) : uint8 = UInt U8 x
+
+let u16 (x:UInt16.t) : uint16 = UInt U16 x
+
+let u32 (x:UInt32.t) : uint32 = UInt U32 x
+
+let u64 (x:UInt64.t) : uint64 = UInt U64 x
+
+let u128 (x:UInt128.t) : uint128 = UInt U128 x
+
+let add_mod a b =
+  match a,b with
+  | UInt U8 a, UInt U8 b -> UInt U8 (UInt8.add_mod a b)
+  | UInt U16 a, UInt U16 b -> UInt U16 (UInt16.add_mod a b)
+  | UInt U32 a, UInt U32 b -> UInt U32 (UInt32.add_mod a b)
+  | UInt U64 a, UInt U64 b -> UInt U64 (UInt64.add_mod a b)
+  | UInt U128 a, UInt U128 b -> UInt U128 (UInt128.add_mod a b)
+  
+
+let add a b = 
+  match a,b with
+  | UInt U8 a, UInt U8 b -> UInt U8 (UInt8.add a b)
+  | UInt U16 a, UInt U16 b -> UInt U16 (UInt16.add a b)
+  | UInt U32 a, UInt U32 b -> UInt U32 (UInt32.add a b)
+  | UInt U64 a, UInt U64 b -> UInt U64 (UInt64.add a b)
+  | UInt U128 a, UInt U128 b -> UInt U128 (UInt128.add a b)
+
+
+//#reset-options "--z3rlimit 50"
+
+let mul_mod a b = 
+  match a,b with
+  | UInt U8 a, UInt U8 b -> UInt U8 (UInt8.mul_mod a b)
+  | UInt U16 a, UInt U16 b -> UInt U16 (UInt16.mul_mod a b)
+  | UInt U32 a, UInt U32 b -> UInt U32 (UInt32.mul_mod a b)
+  | UInt U64 a, UInt U64 b -> UInt U64 (UInt64.mul_mod a b)
+
+
+let mul a b = 
+  match a,b with
+  | UInt U8 a, UInt U8 b -> UInt U8 (UInt8.mul a b)
+  | UInt U16 a, UInt U16 b -> UInt U16 (UInt16.mul a b)
+  | UInt U32 a, UInt U32 b -> UInt U32 (UInt32.mul a b)
+  | UInt U64 a, UInt U64 b -> UInt U64 (UInt64.mul a b)
+
+
+let sub_mod a b = 
+  match a,b with
+  | UInt U8 a, UInt U8 b -> UInt U8 (UInt8.sub_mod a b)
+  | UInt U16 a, UInt U16 b -> UInt U16 (UInt16.sub_mod a b)
+  | UInt U32 a, UInt U32 b -> UInt U32 (UInt32.sub_mod a b)
+  | UInt U64 a, UInt U64 b -> UInt U64 (UInt64.sub_mod a b)
+  | UInt U128 a, UInt U128 b -> UInt U128 (UInt128.sub_mod a b)
+
+
+let sub a b = 
+  match a,b with
+  | UInt U8 a, UInt U8 b -> UInt U8 (UInt8.sub a b)
+  | UInt U16 a, UInt U16 b -> UInt U16 (UInt16.sub a b)
+  | UInt U32 a, UInt U32 b -> UInt U32 (UInt32.sub a b)
+  | UInt U64 a, UInt U64 b -> UInt U64 (UInt64.sub a b)
+  | UInt U128 a, UInt U128 b -> UInt U128 (UInt128.sub a b)
+
+
+let logxor a b = 
+  match a,b with
+  | UInt U8 a, UInt U8 b -> UInt U8 (UInt8.logxor a b)
+  | UInt U16 a, UInt U16 b -> UInt U16 (UInt16.logxor a b)
+  | UInt U32 a, UInt U32 b -> UInt U32 (UInt32.logxor a b)
+  | UInt U64 a, UInt U64 b -> UInt U64 (UInt64.logxor a b)
+  | UInt U128 a, UInt U128 b -> UInt U128 (UInt128.logxor a b)
+
+
+let logand a b = 
+  match a,b with
+  | UInt U8 a, UInt U8 b -> UInt U8 (UInt8.logand a b)
+  | UInt U16 a, UInt U16 b -> UInt U16 (UInt16.logand a b)
+  | UInt U32 a, UInt U32 b -> UInt U32 (UInt32.logand a b)
+  | UInt U64 a, UInt U64 b -> UInt U64 (UInt64.logand a b)
+  | UInt U128 a, UInt U128 b -> UInt U128 (UInt128.logand a b)
+
+
+let logor a b = 
+  match a,b with
+  | UInt U8 a, UInt U8 b -> UInt U8 (UInt8.logor a b)
+  | UInt U16 a, UInt U16 b -> UInt U16 (UInt16.logor a b)
+  | UInt U32 a, UInt U32 b -> UInt U32 (UInt32.logor a b)
+  | UInt U64 a, UInt U64 b -> UInt U64 (UInt64.logor a b)
+  | UInt U128 a, UInt U128 b -> UInt U128 (UInt128.logor a b)
+
+
+let lognot a = 
+  match a with
+  | UInt U8 a -> UInt U8 (UInt8.lognot a)
+  | UInt U16 a -> UInt U16 (UInt16.lognot a)
+  | UInt U32 a -> UInt U32 (UInt32.lognot a)
+  | UInt U64 a -> UInt U64 (UInt64.lognot a)
+  | UInt U128 a -> UInt U128 (UInt128.lognot a)
+
+
+let shift_right a b = 
+  match a with
+  | UInt U8 a -> UInt U8 (UInt8.shift_right a b)
+  | UInt U16 a -> UInt U16 (UInt16.shift_right a b)
+  | UInt U32 a -> UInt U32 (UInt32.shift_right a b)
+  | UInt U64 a -> UInt U64 (UInt64.shift_right a b)
+  | UInt U128 a -> UInt U128 (UInt128.shift_right a b)
+
+
+let shift_left a b = 
+  match a with
+  | UInt U8 a -> UInt U8 (UInt8.shift_left a b)
+  | UInt U16 a -> UInt U16 (UInt16.shift_left a b)
+  | UInt U32 a -> UInt U32 (UInt32.shift_left a b)
+  | UInt U64 a -> UInt U64 (UInt64.shift_left a b)
+  | UInt U128 a -> UInt U128 (UInt128.shift_left a b)
+
+
+let rotate_right a b = 
+  (logor (shift_right a b)  (shift_left a (UInt32.uint_to_t (bits a.t - UInt32.v b))))
+
+
+let rotate_left a b = 
+  (logor (shift_left a b)  (shift_right a (UInt32.uint_to_t (bits a.t - UInt32.v b))))
+
+
+let eq_mask a b = 
+  match a,b with
+  | UInt U8 a, UInt U8 b -> if FStar.UInt8.(a =^ b) then (u8 0xffuy) else (u8 0uy)
+  | UInt U16 a, UInt U16 b -> if FStar.UInt16.(a =^ b) then (u16 0xffffus) else (u16 0us)
+  | UInt U32 a, UInt U32 b -> if FStar.UInt32.(a =^ b) then (u32 0xfffffffful) else (u32 0ul) 
+  | UInt U64 a, UInt U64 b -> if FStar.UInt64.(a =^ b) then (u64 0xffffffffffffffffuL) else (u64 0uL) 
+  | UInt U128 a, UInt U128 b -> if FStar.UInt128.(a =^ b) then (u128 (FStar.UInt128.uint_to_t 0xffffffffffffffffffffffffffffffff)) else (u128 (FStar.UInt128.uint_to_t 0))
+
+let neq_mask a b = 
+  match a,b with
+  | UInt U8 a, UInt U8 b -> if not FStar.UInt8.(a =^ b) then (u8 0xffuy) else (u8 0uy)
+  | UInt U16 a, UInt U16 b -> if not FStar.UInt16.(a =^ b) then (u16 0xffffus) else (u16 0us)
+  | UInt U32 a, UInt U32 b -> if not FStar.UInt32.(a =^ b) then (u32 0xfffffffful) else (u32 0ul) 
+  | UInt U64 a, UInt U64 b -> if not FStar.UInt64.(a =^ b) then (u64 0xffffffffffffffffuL) else (u64 0uL) 
+  | UInt U128 a, UInt U128 b -> if not FStar.UInt128.(a =^ b) then (u128 (FStar.UInt128.uint_to_t 0xffffffffffffffffffffffffffffffff)) else (u128 (FStar.UInt128.uint_to_t 0))
+
+let gte_mask a b = 
+  match a,b with
+  | UInt U8 a, UInt U8 b -> if FStar.UInt8.(a >=^ b) then (u8 0xffuy) else (u8 0uy)
+  | UInt U16 a, UInt U16 b -> if FStar.UInt16.(a >=^ b) then (u16 0xffffus) else (u16 0us)
+  | UInt U32 a, UInt U32 b -> if FStar.UInt32.(a >=^ b) then (u32 0xfffffffful) else (u32 0ul) 
+  | UInt U64 a, UInt U64 b -> if FStar.UInt64.(a >=^ b) then (u64 0xffffffffffffffffuL) else (u64 0uL) 
+  | UInt U128 a, UInt U128 b -> if FStar.UInt128.(a >=^ b) then (u128 (FStar.UInt128.uint_to_t 0xffffffffffffffffffffffffffffffff)) else (u128 (FStar.UInt128.uint_to_t 0))
+
+let gt_mask a b = 
+  match a,b with
+  | UInt U8 a, UInt U8 b -> if FStar.UInt8.(a >^ b) then (u8 0xffuy) else (u8 0uy)
+  | UInt U16 a, UInt U16 b -> if FStar.UInt16.(a >^ b) then (u16 0xffffus) else (u16 0us)
+  | UInt U32 a, UInt U32 b -> if FStar.UInt32.(a >^ b) then (u32 0xfffffffful) else (u32 0ul) 
+  | UInt U64 a, UInt U64 b -> if FStar.UInt64.(a >^ b) then (u64 0xffffffffffffffffuL) else (u64 0uL) 
+  | UInt U128 a, UInt U128 b -> if FStar.UInt128.(a >^ b) then (u128 (FStar.UInt128.uint_to_t 0xffffffffffffffffffffffffffffffff)) else (u128 (FStar.UInt128.uint_to_t 0))
+
+
+let lt_mask a b = 
+  match a,b with
+  | UInt U8 a, UInt U8 b -> if FStar.UInt8.(a <^ b) then (u8 0xffuy) else (u8 0uy)
+  | UInt U16 a, UInt U16 b -> if FStar.UInt16.(a <^ b) then (u16 0xffffus) else (u16 0us)
+  | UInt U32 a, UInt U32 b -> if FStar.UInt32.(a <^ b) then (u32 0xfffffffful) else (u32 0ul) 
+  | UInt U64 a, UInt U64 b -> if FStar.UInt64.(a <^ b) then (u64 0xffffffffffffffffuL) else (u64 0uL) 
+  | UInt U128 a, UInt U128 b -> if FStar.UInt128.(a <^ b) then (u128 (FStar.UInt128.uint_to_t 0xffffffffffffffffffffffffffffffff)) else (u128 (FStar.UInt128.uint_to_t 0))
+
+let lte_mask a b = 
+  match a,b with
+  | UInt U8 a, UInt U8 b -> if FStar.UInt8.(a <=^ b) then (u8 0xffuy) else (u8 0uy)
+  | UInt U16 a, UInt U16 b -> if FStar.UInt16.(a <=^ b) then (u16 0xffffus) else (u16 0us)
+  | UInt U32 a, UInt U32 b -> if FStar.UInt32.(a <=^ b) then (u32 0xfffffffful) else (u32 0ul) 
+  | UInt U64 a, UInt U64 b -> if FStar.UInt64.(a <=^ b) then (u64 0xffffffffffffffffuL) else (u64 0uL) 
+  | UInt U128 a, UInt U128 b -> if FStar.UInt128.(a <=^ b) then (u128 (FStar.UInt128.uint_to_t 0xffffffffffffffffffffffffffffffff)) else (u128 (FStar.UInt128.uint_to_t 0))
+ 
+(* defined in .fsti: notations +^, -^, ...*)
+
+type bignum = nat
+let bn_v n = n
+let bn n = n
+let bn_add a b = a + b
+let bn_mul a b = a `op_Multiply` b
+let bn_sub a b = a - b
+let bn_mod a b = a % b
+let bn_div a b = a / b
+
